% Equations dictionary

\documentclass[11pt]{article}
\usepackage{amsmath,eqparbox,xparse,mathtools}

% load macros
\usepackage{macros}

% Begin document
\begin{document}

%<*eqstate>
\begin{subequations}
\label{e:state}
\begin{align}
\Phi &= \left\{T, V, n_1, n_2 \ldots n_{\ns/ - 1}\right\}&\text{\dconp/,}\\
\Phi &= \left\{T, P, n_1, n_2 \ldots n_{\ns/ - 1}\right\}&\text{\dconv/,}
\end{align}
\end{subequations}
%</eqstate>

%<*eqdstate>
\begin{subequations}
\label{e:source_terms}
\begin{align}
f &= \frac{\text{d} \Phi }{\text{d} t } = \left\{\frac{\text{d} T }{\text{d} t },\frac{\text{d} V }{\text{d} t },\frac{\text{d} n_1}{\text{d} t },\frac{\text{d} n_2 }{\text{d} t }\ldots \frac{\text{d} n_{\ns/ - 1} }{\text{d} t }\right\} & \text{\dconp/,} \\
f &= \frac{\text{d} \Phi }{\text{d} t } = \left\{\frac{\text{d} T }{\text{d} t },\frac{\text{d} P }{\text{d} t },\frac{\text{d} n_1}{\text{d} t },\frac{\text{d} n_2 }{\text{d} t }\ldots \frac{\text{d} n_{\ns/ - 1} }{\text{d} t }\right\} & \text{\dconv/.}
\end{align}
\end{subequations}
%</eqdstate>

%<*eqdmolar>
\begin{equation}
\label{e:spec}
\frac{\text{d} n_{k} }{\text{d} t } = V \dot{\omega}_{k} \qquad k = 1, \ldots, \ns/ - 1,
\end{equation}
%</eqdmolar>

%<*eqdTdotdT>
\begin{subequations}
\label{e:dTdotdT}
\begin{align}
\mathcal{J}_{1, 1} &= \frac{1}{\sum_{k=1}^{\ns/} [C]_{k} {C_p}_{k}} \Biggl[ \frac{\text{d} T }{\text{d} t } \sum_{k=1}^{\ns/} \left(- \frac{\text{d} {C_p} }{\text{d} T }_{k} + \frac{{C_p}_{\ns/}}{T}\right) [C]_{k} + & \nonumber \\
				    & \sum_{k=1}^{-1 + \ns/} \biggl( \left(- H_{k} + \frac{W_{k} H_{\ns/}}{W_{\ns/}}\right) \frac{\mathcal{J}_{k + 2, 1}}{V} + & \nonumber \\
				    & \mathindent[larger] \left(- {C_p}_{k} + \frac{W_{k} {C_p}_{k} }{W_{\ns/}} \right) \dot{\omega}_{k}\biggr)\Biggr] & \text{\dconp/,} \\
\intertext{and similarly:}
\mathcal{J}_{1, 1} &= \frac{1}{\sum_{k=1}^{\ns/} [C]_{k} {C_v}_{k}} \Biggl[ \frac{\text{d} T }{\text{d} t } \sum_{k=1}^{\ns/} \left(- \frac{\text{d} {C_v} }{\text{d} T }_{k} + \frac{{C_v}_{\ns/}}{T}\right) [C]_{k} + & \nonumber \\
				     & \sum_{k=1}^{-1 + \ns/} \biggl(\left(- U_{k} + \frac{W_{k} U_{\ns/}}{W_{\ns/}}\right) \frac{\mathcal{J}_{k + 2, 1}}{V} + & \nonumber \\
				     & \mathindent[larger] \left(- {C_v}_{k} + \frac{W_{k} {C_v}_{\ns/}}{W_{\ns/}}\right) \dot{\omega}_{k}\biggr)\Biggr] & \text{\dconv/.}
\end{align}
\end{subequations}
%</eqdTdotdT>

%<*eqdtemp>
\begin{subequations}
\label{e:temperature_incomplete}
\begin{align}
\frac{\text{d} T }{\text{d} t } &= - \frac{\sum_{k=1}^{\ns/} H_{k} \dot{\omega}_{k}}{\sum_{k=1}^{\ns/} [C]_{k} {C_{p, k}}} & \text{\dconp/,} \\
\frac{\text{d} T }{\text{d} t } &= - \frac{\sum_{k=1}^{\ns/} U_{k} \dot{\omega}_{k}}{\sum_{k=1}^{\ns/} [C]_{k} {C_{v, k}}} & \text{\dconv/,}
\end{align}
\end{subequations}
%</eqdtemp>

%<*eqdparam>
\begin{subequations}
\label{e:param_complete}
\begin{align}
\frac{\text{d} V }{\text{d} t } &= V \left(\frac{T \Ru/}{P} \sum_{k=1}^{\ns/  - 1} \left(1 - \frac{W_{k}}{W_{\ns/}}\right) \dot{\omega}_{k} + \frac{1}{T} \frac{\text{d} T }{\text{d} t }\right)& \text{\dconp/,} \\
\frac{\text{d} P }{\text{d} t } &= T \Ru/ \sum_{k=1}^{\ns/  - 1} \left(1 - \frac{W_{k}}{W_{\ns/}}\right) \dot{\omega}_{k} + \frac{P}{T} \frac{\text{d} T }{\text{d} t }&\text{\dconv/.}
\end{align}
\end{subequations}
%</eqdparam>

%<*eqdEdotdT>
\begin{subequations}
\label{e:dEdotdT}
\begin{align}
 \mathcal{J}_{2, 1} &= \frac{\partial }{\partial T } \frac{\text{d} V}{\text{d} t} = \frac{\partial \dot{V} }{\partial T} & \nonumber \\
		    &= \frac{V}{[C]} \sum_{k=1}^{-1 + \ns/} \left(1 - \frac{W_{k}}{W_{\ns/}}\right) \left(\frac{\mathcal{J}_{k + 2, 1}}{V} + \frac{\dot{\omega}_{k}}{T}\right) \nonumber \\
		    &  \mathindent + \frac{V}{T} \left(\mathcal{J}_{1, 1} - \frac{1}{T} \frac{\text{d} T }{\text{d} t }\right) & \text{\dconp/,}
\intertext{and:}
 \mathcal{J}_{2, 1} &= \frac{\partial }{\partial T } \frac{\text{d} V}{\text{d} t} = \frac{\partial \dot{P} }{\partial T} & \nonumber \\
		    &= \Ru/ \sum_{k=1}^{-1 + \ns/} \left(1 - \frac{W_{k}}{W_{\ns/}}\right) \left(T \frac{\mathcal{J}_{k + 2, 1}}{V} + \dot{\omega}_{k}\right) & \nonumber \\
		    & \mathindent + \frac{P}{T} \left(\mathcal{J}_{1, 1}- \frac{1}{T} \frac{\text{d} T }{\text{d} t }\right) & \text{\dconv/.}
\end{align}
\end{subequations}
%</eqdEdotdT>

%<*eqdnkdotdT>
\begin{align}
 \label{e:dnkdotdT}
 \lhs{dnkdotdT}{\mathcal{J}_{k + 2, 1}}  &= \rhs{dnkdotdT}{V \sum_{i=1}^{\nr/} \left(\nu_{k,i} R_{i} \frac{\partial c_{i}}{\partial T } + \nu_{k,i} \frac{\partial R_{i}}{\partial T } c_{i}\right)} & \cond{dnkdotdT}{,}
\end{align}
%</eqdnkdotdT>

%<*eqdTdotdE>
\begin{subequations}
\label{e:dTdotdE}
\begin{align}
 \mathcal{J}_{1, 2} &= \frac{1}{\sum_{k=1}^{\ns/} V [C]_{k} {C_p}_{k}} \Biggl[ & \nonumber \\
				     & \mathindent - \sum_{k=1}^{-1 + \ns/} \left(H_{k} - \frac{W_{k} H_{\ns/}}{W_{\ns/}}\right) \left(\mathcal{J}_{k + 2, 2} - \dot{\omega}_{k}\right) + & \nonumber \\
				     & \mathindent \frac{\text{d} T }{\text{d} t } \sum_{k=1}^{-1 + \ns/} \left(- {C_p}_{\ns/} + {C_p}_{k}\right) [C]_{k}\Biggr] & \text{\dconp/,} \\
 \mathcal{J}_{1, 2} &= \frac{1}{\sum_{k=1}^{\ns/} [C]_{k} {C_v}_{k}} \Biggl[ & \nonumber \\
				     & \mathindent - \sum_{k=1}^{-1 + \ns/} \left(U_{k} - \frac{W_{k} U_{\ns/}}{W_{\ns/}}\right) \frac{\mathcal{J}_{k + 2, 2}}{V} - & \nonumber \\
				     & \mathindent \frac{{C_v}_{\ns/}}{T \Ru/} \frac{\text{d} T }{\text{d} t } \Biggr] & \text{\dconv/.}
\end{align}
\end{subequations}
%</eqdTdotdE>

%<*eqdEdotdE>
\begin{subequations}
\label{e:dEdotdE}
\begin{align}
 \mathcal{J}_{2, 2} &= \frac{1}{[C]} \sum_{k=1}^{-1 + \ns/} \left(1 - \frac{W_{k}}{W_{\ns/}}\right) \mathcal{J}_{k+2, 2} \nonumber \\
		    & \mathindent + \frac{1}{T} \left(V \mathcal{J}_{1, 2} + \dot{T}\right) & \text{\dconp/,} \\
 \intertext{and:}
 \mathcal{J}_{2, 2} &= \frac{T \Ru/}{V} \sum_{k=1}^{-1 + \ns/} \left(1 - \frac{W_{k}}{W_{\ns/}}\right) \mathcal{J}_{k+2, 2} & \nonumber \\
		    & \mathindent + \frac{1}{T} \left(P \mathcal{J}_{1, 2} + \dot{T}\right) & \text{\dconv/.}
\end{align}
\end{subequations}
%</eqdEdotdE>

%<*eqdnkdotdE>
\begin{subequations}
 \label{e:dnkdotdE}
 \begin{align}
  \lhs{dnkdotdE}{\mathcal{J}_{k + 2, 2}} &= \rhs{dnkdotdE}{V \sum_{i=1}^{\nr/} \left(\nu_{k,i} R_{i} \frac{\partial c_{i}}{\partial V } + \nu_{k,i} \frac{\partial R_{i}}{\partial V } c_{i}\right) + \dot{\omega}_{k}} & \cond{dnkdotdE}{\dconp/,}\\
  \lhs{dnkdotdE}{\mathcal{J}_{k + 2, 2}} &= \rhs{dnkdotdE}{V \sum_{i=1}^{\nr/} \left(\nu_{k,i} R_{i} \frac{\partial c_{i}}{\partial P } + \nu_{k,i} \frac{\partial R_{i}}{\partial P } c_{i}\right)} & \cond{dnkdotdE}{\dconv/.}
 \end{align}
\end{subequations}
%</eqdnkdotdE>

%<*eqdTdotdnj>
\begin{subequations}
\label{e:dTdotdnj}
\begin{align}
 \mathcal{J}_{1, j + 2} &= \frac{1}{\sum_{k=1}^{\ns/} V [C]_{k} {C_p}_{k}} \Biggl[ & \nonumber \\
				       & \mathindent[largerindent] - \sum_{k=1}^{-1 + \ns/} \left(H_{k} - \frac{W_{k} H_{\ns/}}{W_{\ns/}}\right) \mathcal{J}_{k+2, j+2} & \nonumber \\
				       & \mathindent[largerindent] - \frac{\text{d} T }{\text{d} t } \left(- {C_p}_{\ns/} + {C_p}_{j}\right)\Biggr] & \text{\dconp/,} \\
\intertext{and:}
 \mathcal{J}_{1, j + 2} &= \frac{1}{\sum_{k=1}^{\ns/} V [C]_{k} {C_v}_{k}} \Biggl[ & \nonumber \\
				       & \mathindent[largerindent] - \sum_{k=1}^{-1 + \ns/} \left(U_{k} - \frac{W_{k} U_{\ns/}}{W_{\ns/}}\right) \mathcal{J}_{k+2, j+2} & \nonumber \\
				       & \mathindent[largerindent] - \frac{\text{d} T }{\text{d} t } \left(- {C_v}_{\ns/} + {C_v}_{j}\right) \Biggr] & \text{\dconv/.}
\end{align}
\end{subequations}
%</eqdTdotdnj>

%<*eqdEdotdnj>
\begin{subequations}
\label{e:dnkdotdE_nojac}
\begin{align}
 \mathcal{J}_{2, j + 2} &= \frac{1}{[C]} \sum_{k=1}^{-1 + \ns/} \left(1 - \frac{W_{k}}{W_{\ns/}}\right) \mathcal{J}_{k + 2, j + 2} + \frac{V}{T} \mathcal{J}_{1, j + 2} & \text{\dconp/,}
\intertext{and:}
 \mathcal{J}_{2, j + 2} &= \frac{T \Ru/}{V} \sum_{k=1}^{-1 + \ns/} \left(1 - \frac{W_{k}}{W_{\ns/}}\right) \mathcal{J}_{k + 2, j + 2} + \frac{P}{T} \mathcal{J}_{2, j + 2} & \text{\dconv/.}
\end{align}
\end{subequations}
%</eqdEdotdnj>

%<*eqdnkdotdnj>
\begin{align}
 \label{e:dnkdotdnj}
 \lhs{dnkdotdnj}{\mathcal{J}_{k + 2, j + 2}} &= \rhs{dnkdotdnj}{V \sum_{i=1}^{\nr/} \left(\nu_{k,i} R_{i} \frac{\partial c_{i} }{\partial {n_j} } + \nu_{k,i} \frac{\partial R_{i} }{\partial {n_j} } c_{i}\right)} & \cond{dnkdotdnj}{.}
\end{align}
%</eqdnkdotdnj>

%<*eqjacgeneral>
\begin{equation}
 \label{e:jac_general}
 \mathcal{J}_{i,j} = \frac{\partial f_i}{\partial \Phi_j},\qquad i,j=1 \ldots \ns/ - 1\;,
\end{equation}
%</eqjacgeneral>

\end{document}
