\documentclass[a4paper,10pt]{article}
\usepackage[utf8]{inputenc}
\usepackage{amsmath}
\begin{document}
\begin{equation}\bar{W} = \sum_{i=1}^{N_s} W_{i} X_{i}\end{equation}
\begin{equation}n{\left (t \right )} = \frac{m}{\sum_{i=1}^{N_s} W_{i} X_{i}}\end{equation}
\begin{equation}{c_p}_{i} = \bar{R} \left(T \left(T \left(T \left(T a_{i,4} + a_{i,3}\right) + a_{i,2}\right) + a_{i,1}\right) + a_{i,0}\right)\end{equation}
\begin{equation}\frac{\text{d} {c_p} }{\text{d} T }_{i} = \bar{R} \left(T \left(T \left(T a_{i,4} + a_{i,3}\right) + a_{i,2}\right) + T \left(T \left(T a_{i,4} + a_{i,3}\right) + T \left(2 T a_{i,4} + a_{i,3}\right) + a_{i,2}\right) + a_{i,1}\right)\end{equation}
\begin{equation}h_{i} = T \bar{R} \left(T \left(T \left(T \left(0.2 T a_{i,4} + 0.25 a_{i,3}\right) + 0.333333333333333 a_{i,2}\right) + 0.5 a_{i,1}\right) + a_{i,0}\right)\end{equation}
\begin{equation}\frac{\text{d} h }{\text{d} T }_{i} = T \bar{R} \left(T \left(T \left(0.2 T a_{i,4} + 0.25 a_{i,3}\right) + 0.333333333333333 a_{i,2}\right) + T \left(T \left(0.2 T a_{i,4} + 0.25 a_{i,3}\right) + T \left(0.4 T a_{i,4} + 0.25 a_{i,3}\right) + 0.333333333333333 a_{i,2}\right) + 0.5 a_{i,1}\right) + \bar{R} \left(T \left(T \left(T \left(0.2 T a_{i,4} + 0.25 a_{i,3}\right) + 0.333333333333333 a_{i,2}\right) + 0.5 a_{i,1}\right) + a_{i,0}\right)\end{equation}
\begin{equation}B_{i} = T \left(T \left(T \left(\frac{T a_{i,4}}{20} + \frac{a_{i,3}}{12}\right) + \frac{a_{i,2}}{6}\right) + \frac{a_{i,1}}{2}\right) + \left(a_{i,0} - 1\right) \log{\left (T \right )} - a_{i,0} + a_{i,6} - \frac{a_{i,5}}{T}\end{equation}
\begin{equation}\frac{\text{d} B }{\text{d} T }_{i} = T \left(T \left(\frac{T a_{i,4}}{20} + \frac{a_{i,3}}{12}\right) + \frac{a_{i,2}}{6}\right) + T \left(T \left(\frac{T a_{i,4}}{20} + \frac{a_{i,3}}{12}\right) + T \left(\frac{T a_{i,4}}{10} + \frac{a_{i,3}}{12}\right) + \frac{a_{i,2}}{6}\right) + \frac{a_{i,1}}{2} + \frac{1}{T} \left(a_{i,0} - 1\right) + \frac{a_{i,5}}{T^{2}}\end{equation}
\begin{equation}\Phi = \left\{T, [X]_1, [X]_2, \ldots [X]_{N_{sp}}\right\}^{T}\end{equation}
\begin{equation}\frac{\partial \Phi}{\partial t} = \left\{\frac{\partial T}{\partial t}, \frac{\partial [X]_1}{\partial t}, \frac{\partial [X]_2}{\partial t}, \ldots \frac{\partial [X]_{N_{sp}}}{\partial t}\right\}^{T}\end{equation}
\begin{equation}[X] = \frac{P}{T \bar{R}}\end{equation}
\begin{equation}X_{N_s} = - \sum_{i=1}^{-1 + N_s} X + \frac{P}{T \bar{R}}\end{equation}
\begin{equation}\frac{d}{d t} U{\left (t \right )} = - \frac{\text{d} V }{\text{d} t } P\end{equation}
\begin{equation}H{\left (t \right )} = \frac{m \sum_{i=1}^{N_s} X_{i} h_{i}}{\sum_{i=1}^{N_s} W_{i} X_{i}}\end{equation}
\begin{equation}\frac{d}{d t} H{\left (t \right )} = \frac{\text{d} V }{\text{d} t } P + \frac{d}{d t} U{\left (t \right )}\end{equation}
\begin{equation}\frac{d}{d t} U{\left (t \right )} = - \frac{\text{d} V }{\text{d} t } P + \frac{d}{d t} H{\left (t \right )}\end{equation}
\begin{equation}\frac{d}{d t} H{\left (t \right )} = 0\end{equation}
\begin{equation}\frac{m}{\sum_{i=1}^{N_s} W_{i} X_{i}} \sum_{i=1}^{N_s} \left(\frac{\text{d} T }{\text{d} t } X_{i} \frac{\text{d} h }{\text{d} T }_{i} + \frac{\text{d} X }{\text{d} t }_{i} h_{i}\right) - \frac{m}{\left(\sum_{i=1}^{N_s} W_{i} X_{i}\right)^{2}} \left(\sum_{i=1}^{N_s} W_{i} \frac{\text{d} X }{\text{d} t }_{i}\right) \sum_{i=1}^{N_s} X_{i} h_{i} = 0\end{equation}
\begin{equation}\frac{\text{d} T }{\text{d} t } = - \frac{1}{\left(\sum_{i=1}^{N_s} W_{i} X_{i}\right) \sum_{i=1}^{N_s} X_{i} \frac{\text{d} h }{\text{d} T }_{i}} \left(\left(\sum_{i=1}^{N_s} W_{i} X_{i}\right) \sum_{i=1}^{N_s} \frac{\text{d} X }{\text{d} t }_{i} h_{i} - \left(\sum_{i=1}^{N_s} W_{i} \frac{\text{d} X }{\text{d} t }_{i}\right) \sum_{i=1}^{N_s} X_{i} h_{i}\right)\end{equation}
\begin{equation}\frac{\partial\dot{T}}{\partial{X_j}} = \frac{1}{\left(\left(\sum_{i=1}^{N_s} W_{i} X_{i}\right)^{2}\right) \left(\sum_{i=1}^{N_s} X_{i} \frac{\text{d} h }{\text{d} T }_{i}\right)^{2}} \left(- \left(\sum_{i=1}^{N_s} \delta_{i j} W_{i}\right) \left(\sum_{i=1}^{N_s} W_{i} \frac{\text{d} X }{\text{d} t }_{i}\right) \left(\sum_{i=1}^{N_s} X_{i} \frac{\text{d} h }{\text{d} T }_{i}\right) \sum_{i=1}^{N_s} X_{i} h_{i} + \left(\sum_{i=1}^{N_s} \delta_{i j} \frac{\text{d} h }{\text{d} T }_{i}\right) \left(\left(\sum_{i=1}^{N_s} W_{i} X_{i}\right)^{2}\right) \sum_{i=1}^{N_s} \frac{\text{d} X }{\text{d} t }_{i} h_{i} - \left(\sum_{i=1}^{N_s} \delta_{i j} \frac{\text{d} h }{\text{d} T }_{i}\right) \left(\sum_{i=1}^{N_s} W_{i} X_{i}\right) \left(\sum_{i=1}^{N_s} W_{i} \frac{\text{d} X }{\text{d} t }_{i}\right) \sum_{i=1}^{N_s} X_{i} h_{i} + \left(\sum_{i=1}^{N_s} \delta_{i j} h_{i}\right) \left(\sum_{i=1}^{N_s} W_{i} X_{i}\right) \left(\sum_{i=1}^{N_s} W_{i} \frac{\text{d} X }{\text{d} t }_{i}\right) \sum_{i=1}^{N_s} X_{i} \frac{\text{d} h }{\text{d} T }_{i}\right)\end{equation}
\begin{equation}\frac{\partial\dot{T}}{\partial{T}} = \frac{1}{\left(\sum_{i=1}^{N_s} W_{i} X_{i}\right) \left(\sum_{i=1}^{N_s} X_{i} \frac{\text{d} h }{\text{d} T }_{i}\right)^{2}} \left(\left(- \left(\sum_{i=1}^{N_s} W_{i} X_{i}\right) \sum_{i=1}^{N_s} \frac{\text{d} X }{\text{d} t }_{i} \frac{\text{d} h }{\text{d} T }_{i} + \left(\sum_{i=1}^{N_s} W_{i} \frac{\text{d} X }{\text{d} t }_{i}\right) \sum_{i=1}^{N_s} X_{i} \frac{\text{d} h }{\text{d} T }_{i}\right) \sum_{i=1}^{N_s} X_{i} \frac{\text{d} h }{\text{d} T }_{i} + \left(\left(\sum_{i=1}^{N_s} W_{i} X_{i}\right) \sum_{i=1}^{N_s} \frac{\text{d} X }{\text{d} t }_{i} h_{i} - \left(\sum_{i=1}^{N_s} W_{i} \frac{\text{d} X }{\text{d} t }_{i}\right) \sum_{i=1}^{N_s} X_{i} h_{i}\right) \sum_{i=1}^{N_s} X_{i} \frac{\text{d} \frac{\text{d} h }{\text{d} T } }{\text{d} T }_{i}\right)\end{equation}
\begin{equation}{k_f}_{j} = T^{b_{j}} e^{- \frac{{E_{a}}_{j}}{T \bar{R}}} A_{j}\end{equation}
\begin{equation}\frac{\text{d} {k_f} }{\text{d} T }_{j} = \frac{T^{b_{j}} A_{j}}{T} e^{- \frac{{E_{a}}_{j}}{T \bar{R}}} b_{j} + \frac{T^{b_{j}} A_{j} {E_{a}}_{j}}{T^{2} \bar{R}} e^{- \frac{{E_{a}}_{j}}{T \bar{R}}}\end{equation}
\begin{equation}\nu_{i,j} = - \nu^{\prime\prime}_{i,j} + \nu^{\prime}_{i,j}\end{equation}
\begin{equation}{K_c}_{j} = \left(\left(\frac{P}{T}\right)^{\sum_{i=1}^{N_s} \nu_{i,j}}\right) e^{\sum_{i=1}^{N_s} \nu_{i,j} B_{i}}\end{equation}
\begin{equation}\frac{\text{d} {K_c} }{\text{d} T }_{j} = \frac{1}{T} \left(\left(\frac{P}{T}\right)^{\sum_{i=1}^{N_s} \nu_{i,j}}\right) \left(T \sum_{i=1}^{N_s} \nu_{i,j} \frac{\text{d} B }{\text{d} T }_{i} - \sum_{i=1}^{N_s} \nu_{i,j}\right) e^{\sum_{i=1}^{N_s} \nu_{i,j} B_{i}}\end{equation}
\begin{equation}{R_{net}}_{j} = {k_f}_{j} \prod_{i=1}^{N_s} X_{i}^{\nu^{\prime}_{i,j}} - \frac{{k_f}_{j}}{{K_c}_{j}} \prod_{i=1}^{N_s} X_{i}^{\nu^{\prime\prime}_{i,j}}\end{equation}
\begin{equation}\frac{\text{d} X }{\text{d} t }_{i} = \sum_{j=1}^{N_r} \left({k_f}_{j} \prod_{i=1}^{N_s} X_{i}^{\nu^{\prime}_{i,j}} - \frac{{k_f}_{j}}{{K_c}_{j}} \prod_{i=1}^{N_s} X_{i}^{\nu^{\prime\prime}_{i,j}}\right)\end{equation}
\begin{equation}\delta_{j k} \frac{\partial \dot{X} }{\partial X[k] }_{i} = \sum_{j=1}^{N_r} \left({k_f}_{j} \prod_{i=1}^{N_s} \frac{\nu^{\prime}_{i,j} X_{i}^{\nu^{\prime}_{i,j}}}{X_{i}} \delta_{i k} - \frac{{k_f}_{j}}{{K_c}_{j}} \prod_{i=1}^{N_s} \frac{\nu^{\prime\prime}_{i,j} X_{i}^{\nu^{\prime\prime}_{i,j}}}{X_{i}} \delta_{i k}\right)\end{equation}
\begin{equation}\frac{\partial \dot{X} }{\partial T }_{i} = \sum_{j=1}^{N_r} \left(\frac{{k_f}_{j}}{{K_c}_{j}^{2}} \frac{\text{d} {K_c} }{\text{d} T }_{j} \prod_{i=1}^{N_s} X_{i}^{\nu^{\prime\prime}_{i,j}} + \frac{\text{d} {k_f} }{\text{d} T }_{j} \prod_{i=1}^{N_s} X_{i}^{\nu^{\prime}_{i,j}} - \frac{1}{{K_c}_{j}} \frac{\text{d} {k_f} }{\text{d} T }_{j} \prod_{i=1}^{N_s} X_{i}^{\nu^{\prime\prime}_{i,j}}\right)\end{equation}
\end{document}
